theories/compiler/prelude.v
@@ -27,7 +27,6 @@ Record module_runtime :=
 Record function_env :=
   { fe_type_vars : list kind;
     fe_return : list type;
-    fe_params : list (list primitive);
     fe_locals : list (list primitive)
   }.
 
@@ -39,20 +38,19 @@ Inductive error :=
 | ETodo.
 
 Definition fe_of_module_func (mf : module_function) : option function_env :=
-  ηss_locals ← mapM eval_rep_prim_empty mf.(mf_locals);
   let ϕ := flatten_function_type mf.(mf_type) in
   ρs ← mapM (type_rep ϕ.(fft_type_vars)) ϕ.(fft_in);
-  ηss_params ← mapM eval_rep_prim_empty ρs;
-  Some (Build_function_env ϕ.(fft_type_vars) ϕ.(fft_out) ηss_params ηss_locals).
+  ηss_P ← mapM eval_rep_prim_empty ρs;
+  ηss_L ← mapM eval_rep_prim_empty mf.(mf_locals);
+  Some (Build_function_env ϕ.(fft_type_vars) ϕ.(fft_out) (ηss_P ++ ηss_L)).
 
 Definition fe_of_context (F : function_ctx) : function_env :=
   {| fe_type_vars := F.(fc_type_vars);
      fe_return := F.(fc_return);
-     fe_params := F.(fc_params);
      fe_locals := F.(fc_locals) |}.
 
 Definition fe_wlocal_offset (fe : function_env) : nat :=
-  sum_list_with length (fe.(fe_params) ++ fe.(fe_locals)).
+  sum_list_with length fe.(fe_locals).
 
 Definition offset_mm : W.static_offset := 3%N.
 Definition offset_gc : W.static_offset := 1%N.
